Weidenbach_Book/CDCL_W_Full.thy
@@ -6,13 +6,13 @@ context conflict_driven_clause_learning\<^sub>W
 begin
 lemma rtranclp_cdcl\<^sub>W_merge_stgy_distinct_mset_clauses:
   assumes invR: "cdcl\<^sub>W_all_struct_inv R" and
-  st: "cdcl\<^sub>W_merge_stgy\<^sup>*\<^sup>* R S" and
+  st: "cdcl\<^sub>W_s'\<^sup>*\<^sup>* R S" and
   dist: "distinct_mset (clauses R)" and
   R: "trail R = []"
   shows "distinct_mset (clauses S)"
   using rtranclp_cdcl\<^sub>W_stgy_distinct_mset_clauses[OF invR _ dist R]
   invR st rtranclp_mono[of cdcl\<^sub>W_s' "cdcl\<^sub>W_stgy\<^sup>*\<^sup>*"] cdcl\<^sub>W_s'_is_rtranclp_cdcl\<^sub>W_stgy
-  by (auto dest!: cdcl\<^sub>W_s'_is_rtranclp_cdcl\<^sub>W_stgy rtranclp_cdcl\<^sub>W_merge_stgy_rtranclp_cdcl\<^sub>W_s')
+  by (auto dest!: cdcl\<^sub>W_s'_is_rtranclp_cdcl\<^sub>W_stgy)
 end
 
 end
